Main.v
@@ -121,6 +121,14 @@ Lemma smt_plus_lemma:
   destruct e1, e2; try unfold symbolize_expr; reflexivity.
  Qed.
 
+ Lemma smt_minus_lemma:
+ forall (e1 e2 : expr),
+ symbolize_expr (Minus e1 e2) = SymMinus (symbolize_expr e1) (symbolize_expr e2).
+ Proof.
+  intros.
+  destruct e1, e2; try unfold symbolize_expr; reflexivity.
+ Qed.
+
 (* Prove that the SMT equivalence checker is correct *)
 Theorem smt_equivalence_checker_correct:
   forall (e1 e2 : expr) (s : state), smt_equivalence_checker e1 e2 s = true -> aequiv e1 e2 s.
@@ -134,10 +142,14 @@ Proof.
     rewrite H.
     reflexivity.
   - unfold smt_equivalence_checker in H.
-    unfold sym_plus in H.
     apply sound_sym_checker.
     rewrite smt_plus_lemma.
     rewrite smt_plus_lemma.
+    apply H.
+  - unfold smt_equivalence_checker in H.
+    apply sound_sym_checker.
+    rewrite smt_minus_lemma.
+    rewrite smt_minus_lemma.
     apply H.
   - unfold smt_equivalence_checker in H.
     apply String.eqb_eq in H.
